src/Syntax/Labelled_Digraph.thy
@@ -16,4 +16,10 @@ where \<open>with_proj' G \<equiv> \<lparr> verts = pverts G,
 definition add_arc :: \<open>[ 'a, 'b, 'a, ('a, 'b) labelled_pair_pre_digraph ] \<Rightarrow> ('a, 'b) labelled_pair_pre_digraph\<close>
 where \<open>add_arc u l v G \<equiv> \<lparr> pverts = pverts G \<union> {u, v}, parcs = insert (u, v) (parcs G), labels = (labels G)((u, v) \<mapsto> l) \<rparr>\<close>
 
+lemma add_arc_no_new_vertex: \<open>\<lbrakk> a \<in> pverts G; b \<in> pverts G \<rbrakk> \<Longrightarrow> pverts (add_arc a l b G) = pverts G\<close>
+  by (auto simp add: add_arc_def)
+
+definition remove_arc :: \<open>[ 'a, 'a, ('a, 'b) labelled_pair_pre_digraph ] \<Rightarrow> ('a, 'b) labelled_pair_pre_digraph\<close>
+where \<open>remove_arc u v G \<equiv> G \<lparr> parcs := parcs G - {(u, v)}, labels := (labels G)((u, v) := None) \<rparr>\<close>
+
 end
